may need to unroll

src/certigrad/aevb/grads_correct.lean
@@ -15,68 +15,18 @@ namespace aevb
 
 open graph list tactic certigrad.tactic
 
-section proof
-parameters (a : arch) (ws : weights a) (x_data : T [a^.n_in, a^.n_x])
-def g := reparam (integrate_kl $ graph_naive a x_data)
-def fdict := mk_input_dict ws g
-
-attribute [cgsimp] g fdict
-
-private meta def prove_indep_hyps : tactic unit :=
-do to_expr ```((g a x_data)^.targets ⊆ env.keys (fdict a ws x_data)) >>= assert `H_tgts_ss_inputs,
-     solve1 cgsimp,
-   to_expr ```(pdfs_exist_at (g a x_data)^.nodes (fdict a ws x_data)) >>= assert `H_pdfs_exist,
-     solve1 cgsimp
-
-private meta def prove_dep_hyps (tgt : expr) : tactic unit :=
-do to_expr ```(well_formed_at (g a x_data)^.costs (g a x_data)^.nodes (fdict a ws x_data) %%tgt) >>= assert `H_wf,
-     focus1 (constructor >> all_goals cgsimp), rotate 1,
-   to_expr ```(grads_exist_at (g a x_data)^.nodes (fdict a ws x_data) %%tgt) >>= assert `H_gs_exist,
-     solve1 (cgsimp),
-   to_expr ```(is_gintegrable (λ m, ⟦compute_grad_slow (g a x_data)^.costs (g a x_data)^.nodes m %%tgt⟧) (fdict a ws x_data) (g a x_data)^.nodes dvec.head) >>= assert `H_gint,
-     solve1 (cgsimp >> prove_is_mvn_integrable),
-   to_expr ```(can_differentiate_under_integrals (g a x_data)^.costs (g a x_data)^.nodes (fdict a ws x_data) %%tgt) >>= assert `H_can_diff,
-     solve1 (cgsimp >> prove_is_mvn_uintegrable)
-
-private meta def forall_idxs (tac_base tac_step : tactic unit) : expr → tactic unit
-| idx :=
-tac_base <|>
-(do cases idx [`_idx],
-    solve1 tac_step,
-    get_local `_idx >>= forall_idxs)
-
-private meta def prove_aevb_base : tactic unit :=
-do exfalso,
-   H_at_idx ← get_local `H_at_idx,
-   to_expr ```(list.at_idx_over %%H_at_idx dec_trivial) >>= exact
-
-private meta def prove_aevb_step : tactic unit :=
-do H_at_idx ← get_local `H_at_idx,
-   mk_app `and.right [H_at_idx] >>= note `H_tgt_eq,
-   H_tgt_eq_type ← get_local `H_tgt_eq >>= infer_type,
-   s ← join_user_simp_lemmas true [`cgsimp],
-   (H_tgt_eq_new_type, pr) ← simplify s H_tgt_eq_type {},
-   get_local `H_tgt_eq >>= λ H_tgt_eq, replace_hyp H_tgt_eq H_tgt_eq_new_type pr,
-   get_local `H_tgt_eq >>= subst,
-   (tgt, new_tgt) ← match_eq H_tgt_eq_new_type,
-   prove_dep_hyps new_tgt,
-   to_expr ```(backprop_correct (fdict a ws x_data) (g a x_data)^.targets H_tgts_ss_inputs H_at_idx H_wf H_gs_exist H_pdfs_exist H_gint H_can_diff) >>= exact
-
-meta def prove_aevb_ok : tactic unit :=
-do -- introduce hypotheses
-   [tgt, idx, H_at_idx] ← intros | fail "can't intro hyps",
-   -- prove independent hyps once and for all
-   prove_indep_hyps,
-   -- repeated case-analysis on idx
-   forall_idxs prove_aevb_base prove_aevb_step idx
-
-lemma aevb_backprop_correct :
+theorem aevb_backprop_correct (a : arch) (ws : weights a) (x_data : T [a^.n_in, a^.n_x]) :
+let g := reparam (integrate_kl $ graph_naive a x_data) in
+let fdict := mk_input_dict ws g in
 ∀ (tgt : reference) (idx : ℕ) (H_at_idx : at_idx g^.targets idx tgt),
 ∇ (λ θ₀, E (graph.to_dist (λ m, ⟦sum_costs m g^.costs⟧) (env.insert tgt θ₀ fdict) g^.nodes) dvec.head) (env.get tgt fdict)
 =
 E (graph.to_dist (λ m, backprop g^.costs g^.nodes m g^.targets) fdict g^.nodes) (λ dict, dvec.get tgt.2 dict idx) :=
-by prove_aevb_ok
+by do whnf_target,
+      g ← to_expr ```(reparam (integrate_kl $ graph_naive a x_data)),
+      fdict ← to_expr ```(mk_input_dict ws (reparam (integrate_kl $ graph_naive a x_data))),
+      prove_model_ok g fdict
 
-end proof
+
 end aevb
 end certigrad
